day05, proof progress

sol/day05_common.v
@@ -49,3 +49,99 @@ Definition react_f (stack : list int) (c : int) : list int :=
 
 Definition react (cs : list int) : list int :=
   fold_left react_f cs [].
+
+Section spec.
+
+Context {A : Type}.
+Context (can_react : A -> A -> Prop).
+
+Variant react_step : list A -> list A -> Prop :=
+| RStep (c1 c2 : A) (cs1 cs2 : list A) :
+    can_react c1 c2 ->
+    react_step (cs1 ++ c1 :: c2 :: cs2) (cs1 ++ cs2).
+
+(* Reflexive transitive closure of [react_step]. *)
+Inductive react_steps : list A -> list A -> Prop :=
+| Steps0 (cs : list A) : react_steps cs cs
+| Steps1 (cs cs' cs'' : list A) :
+    react_step  cs  cs'  ->
+    react_steps cs' cs'' ->
+    react_steps cs  cs''
+.
+
+(* [can_react] should be an involutive function. *)
+Hypothesis can_react_symmetric :
+  forall a b, can_react a b -> can_react b a.
+Hypothesis can_react_function :
+  forall a b c, can_react a b -> can_react a c -> b = c.
+
+Lemma can_react_cofunction :
+  forall a b c, can_react a c -> can_react b c -> a = b.
+Proof.
+  intros; eapply can_react_function, can_react_symmetric; eauto.
+Qed.
+
+Ltac gd xs :=
+  match xs with
+  | (?xs, ?x) => generalize dependent x; gd xs
+  | ?x => generalize dependent x
+  end.
+
+(* The top and left sides of the square imply the right and bottom
+   ones.
+
+     cs0 > cs1
+      v     v
+     cs2 > cs3
+
+ *)
+Lemma react_step_confluent :
+  forall cs0 cs1 cs2,
+    react_step cs0 cs1 -> react_step cs0 cs2 ->
+    cs1 = cs2 \/ (exists cs3,
+                     react_step cs1 cs3 /\ react_step cs2 cs3).
+Proof.
+  intros cs0 cs1 cs2 H01 H02.
+  inversion H01; inversion H02; clear H01 H02.
+  gd (cs1, cs2, c1, c2, cs4, c0, c3, cs5, cs6).
+  induction cs3; simpl; intros.
+  - destruct cs5 as [|c5' cs5]; simpl in *.
+    + left; subst. inversion H3; subst; auto.
+    + destruct cs5; simpl in *.
+      * left; subst. inversion H3; subst. f_equal.
+        eapply can_react_function; eauto.
+      * right; subst. inversion H3; subst.
+        exists (cs5 ++ cs6).
+        split.
+        { apply RStep; auto. }
+        { apply (RStep _ _ []); auto. }
+  - admit.
+Abort.
+
+End spec.
+
+Section example.
+Definition A := 0. Definition a := 1.
+Definition B := 2. Definition b := 3.
+Definition C := 4. Definition c := 5.
+Definition can_react_nat (x y : nat) : Prop := S x = y \/ x = S y.
+Fixpoint react_list (css : list (list nat)) : Prop :=
+  match css with
+  | cs :: (cs' :: _) as css =>
+    react_step can_react_nat cs cs' /\
+    react_list css
+  | _ => True
+  end.
+Example react_ex :
+  react_list
+    [[A;c;C;a;C;B;A;c;C];
+     [A;a;C;B;A;c;C];
+     [C;B;A;c;C];
+     [C;B;A]].
+Proof.
+  repeat constructor.
+  - eapply (RStep _ c C [A]). right;auto.
+  - eapply (RStep _ A a []). left;auto.
+  - eapply (RStep _ c C [_; _; _]). right; auto.
+Qed.
+End example.
